prove weth_inv' up to fsig execution

Blanc/ReSolvent.lean
@@ -877,6 +877,227 @@ lemma Line.inv_solvent {e e' s l s' a}
     (h_sv : Devm.Solvent s a e) (h_run : Line.Run e' s l s') : Devm.Solvent s' a e := by
   unfold Devm.Solvent; rw [← h_bal h_run, ← h_stor h_run]; exact h_sv
 
+def Ninst.Inv {ξ : Type} (r : Devm → ξ) (i : Ninst) : Prop :=
+  ∀ {e s s'}, Ninst.Run e s i s' → r s = r s'
+
+lemma Line.nil_inv {ξ : Type} {f : Devm → ξ} : Line.Inv f [] := by
+  intros e s s' h; cases h; rfl
+
+lemma Line.cons_inv {ξ : Type} {f : Devm → ξ} {i l} :
+    Ninst.Inv f i → Line.Inv f l → Line.Inv f (i :: l) := by
+  intros h0 h1 e s s'' h2
+  rcases Line.of_run_cons h2 with ⟨s', h3, h4⟩
+  apply Eq.trans (h0 h3) (h1 h4)
+
+class Ninst.Hinv {ξ : Type} (f : Devm → ξ) (i : Ninst) where (inv : Ninst.Inv f i)
+
+lemma chargeGas_getBal_eq {cost devm devm'} (h : chargeGas cost devm = .ok devm') : devm.getBal = devm'.getBal := by
+  dsimp [chargeGas] at h
+  split at h <;> try contradiction
+  cases h; rfl
+
+lemma Devm.push_getBal_eq {x devm devm'} (h : Devm.push x devm = .ok devm') : devm.getBal = devm'.getBal := by
+  simp only [Devm.push, bind, Except.bind, Except.assert] at h
+  split at h <;> try contradiction
+  cases h; rfl
+
+lemma chargeGas_getStor_eq {cost devm devm'} (h : chargeGas cost devm = .ok devm') : devm.getStor = devm'.getStor := by
+  dsimp [chargeGas] at h
+  split at h <;> try contradiction
+  cases h; rfl
+
+lemma Devm.push_getStor_eq {x devm devm'} (h : Devm.push x devm = .ok devm') : devm.getStor = devm'.getStor := by
+  simp only [Devm.push, bind, Except.bind, Except.assert] at h
+  split at h <;> try contradiction
+  cases h; rfl
+
+lemma Devm.pop_getBal_eq {devm devm' x} (h : Devm.pop devm = .ok ⟨x, devm'⟩) : devm.getBal = devm'.getBal := by
+  dsimp [Devm.pop] at h; split at h <;> try contradiction
+  cases h; rfl
+
+lemma Devm.pop_getStor_eq {devm devm' x} (h : Devm.pop devm = .ok ⟨x, devm'⟩) : devm.getStor = devm'.getStor := by
+  dsimp [Devm.pop] at h; split at h <;> try contradiction
+  cases h; rfl
+
+lemma pushItem_getBal_eq {x c devm devm'} (h : pushItem x c devm = .ok devm') : devm.getBal = devm'.getBal := by
+  dsimp [pushItem] at h
+  rcases hc : chargeGas c devm with _ | devm2
+  · simp only [hc, bind, Except.bind] at h; contradiction
+  · simp only [hc, bind, Except.bind] at h
+    rcases hp : Devm.push x devm2 with _ | devm3
+    · simp only [hp] at h; contradiction
+    · simp only [hp] at h
+      injection h with h_eq; subst h_eq
+      exact (chargeGas_getBal_eq hc).trans (Devm.push_getBal_eq hp)
+
+lemma pushItem_getStor_eq {x c devm devm'} (h : pushItem x c devm = .ok devm') : devm.getStor = devm'.getStor := by
+  dsimp [pushItem] at h
+  rcases hc : chargeGas c devm with _ | devm2
+  · simp only [hc, bind, Except.bind] at h; contradiction
+  · simp only [hc, bind, Except.bind] at h
+    rcases hp : Devm.push x devm2 with _ | devm3
+    · simp only [hp] at h; contradiction
+    · simp only [hp] at h
+      injection h with h_eq; subst h_eq
+      exact (chargeGas_getStor_eq hc).trans (Devm.push_getStor_eq hp)
+
+instance {x} : Ninst.Hinv Devm.getBal (Ninst.pushB256 x) := ⟨by
+  intros e s s' h
+  rcases h with ⟨xl, h_filled, pc, run⟩
+  cases xl with
+  | some _ => cases run
+  | none =>
+    dsimp [Ninst.Run', Ninst.pushB256] at run
+    rcases hc : chargeGas (if (x.toB8L.sig) = [] then gBase else gVerylow) s with _ | s_gas
+    · rw [hc] at run; dsimp [bind, Except.bind] at run; contradiction
+    · rw [hc] at run; dsimp [bind, Except.bind] at run
+      rcases hp : Devm.push x.toB8L.sig.toB256 s_gas with _ | s''
+      · rw [hp] at run; contradiction
+      · rw [hp] at run
+        injection run with h_eq; subst h_eq
+        exact (chargeGas_getBal_eq hc).trans (Devm.push_getBal_eq hp)
+⟩
+
+instance {x} : Ninst.Hinv Devm.getStor (Ninst.pushB256 x) := ⟨by
+  intros e s s' h
+  rcases h with ⟨xl, h_filled, pc, run⟩
+  cases xl with
+  | some _ => cases run
+  | none =>
+    dsimp [Ninst.Run', Ninst.pushB256] at run
+    rcases hc : chargeGas (if (x.toB8L.sig) = [] then gBase else gVerylow) s with _ | s_gas
+    · rw [hc] at run; dsimp [bind, Except.bind] at run; contradiction
+    · rw [hc] at run; dsimp [bind, Except.bind] at run
+      rcases hp : Devm.push x.toB8L.sig.toB256 s_gas with _ | s''
+      · rw [hp] at run; contradiction
+      · rw [hp] at run
+        injection run with h_eq; subst h_eq
+        exact (chargeGas_getStor_eq hc).trans (Devm.push_getStor_eq hp)
+⟩
+
+instance : Ninst.Hinv Devm.getBal (Ninst.reg Rinst.calldataload) := ⟨by
+  intros e s s' h
+  rcases h with ⟨xl, h_filled, pc, run⟩
+  cases xl with
+  | some _ => cases run
+  | none =>
+    dsimp [Ninst.Run', Rinst.run, Rinst.runCore] at run
+    rcases hp : Devm.pop s with _ | val
+    · rw [hp] at run; dsimp [bind, Except.bind] at run; contradiction
+    · rw [hp] at run; dsimp [bind, Except.bind] at run
+      rcases val with ⟨x1, s1⟩
+      rcases hc : chargeGas gVerylow s1 with _ | s2
+      · rw [hc] at run; dsimp [bind, Except.bind] at run; contradiction
+      · rw [hc] at run; dsimp [bind, Except.bind] at run
+        rcases hpush : Devm.push (B8L.toB256 (List.sliceD e.data x1.toNat 32 0)) s2 with _ | s''
+        · rw [hpush] at run; contradiction
+        · rw [hpush] at run
+          injection run with h_eq; subst h_eq
+          exact (Devm.pop_getBal_eq hp).trans <| (chargeGas_getBal_eq hc).trans (Devm.push_getBal_eq hpush)
+⟩
+
+instance : Ninst.Hinv Devm.getStor (Ninst.reg Rinst.calldataload) := ⟨by
+  intros e s s' h
+  rcases h with ⟨xl, h_filled, pc, run⟩
+  cases xl with
+  | some _ => cases run
+  | none =>
+    dsimp [Ninst.Run', Rinst.run, Rinst.runCore] at run
+    rcases hp : Devm.pop s with _ | val
+    · rw [hp] at run; dsimp [bind, Except.bind] at run; contradiction
+    · rw [hp] at run; dsimp [bind, Except.bind] at run
+      rcases val with ⟨x1, s1⟩
+      rcases hc : chargeGas gVerylow s1 with _ | s2
+      · rw [hc] at run; dsimp [bind, Except.bind] at run; contradiction
+      · rw [hc] at run; dsimp [bind, Except.bind] at run
+        rcases hpush : Devm.push (B8L.toB256 (List.sliceD e.data x1.toNat 32 0)) s2 with _ | s''
+        · rw [hpush] at run; contradiction
+        · rw [hpush] at run
+          injection run with h_eq; subst h_eq
+          exact (Devm.pop_getStor_eq hp).trans <| (chargeGas_getStor_eq hc).trans (Devm.push_getStor_eq hpush)
+⟩
+
+instance : Ninst.Hinv Devm.getBal (Ninst.reg Rinst.shr) := ⟨by
+  intros e s s' h
+  rcases h with ⟨xl, h_filled, pc, run⟩
+  cases xl with
+  | some _ => cases run
+  | none =>
+    dsimp [Ninst.Run', Rinst.run, Rinst.runCore, applyBinary] at run
+    rcases hp1 : Devm.pop s with _ | val1
+    · rw [hp1] at run; dsimp [bind, Except.bind] at run; contradiction
+    · rw [hp1] at run; dsimp [bind, Except.bind] at run
+      rcases val1 with ⟨x1, s1⟩
+      rcases hp2 : Devm.pop s1 with _ | val2
+      · rw [hp2] at run; dsimp [bind, Except.bind] at run; contradiction
+      · rw [hp2] at run; dsimp [bind, Except.bind] at run
+        rcases val2 with ⟨x2, s2⟩
+        rcases hpush : pushItem (x2 >>> x1.toNat) gVerylow s2 with _ | s''
+        · rw [hpush] at run; contradiction
+        · rw [hpush] at run
+          injection run with h_eq; subst h_eq
+          exact (Devm.pop_getBal_eq hp1).trans <| (Devm.pop_getBal_eq hp2).trans <| (pushItem_getBal_eq hpush)
+⟩
+
+instance : Ninst.Hinv Devm.getStor (Ninst.reg Rinst.shr) := ⟨by
+  intros e s s' h
+  rcases h with ⟨xl, h_filled, pc, run⟩
+  cases xl with
+  | some _ => cases run
+  | none =>
+    dsimp [Ninst.Run', Rinst.run, Rinst.runCore, applyBinary] at run
+    rcases hp1 : Devm.pop s with _ | val1
+    · rw [hp1] at run; dsimp [bind, Except.bind] at run; contradiction
+    · rw [hp1] at run; dsimp [bind, Except.bind] at run
+      rcases val1 with ⟨x1, s1⟩
+      rcases hp2 : Devm.pop s1 with _ | val2
+      · rw [hp2] at run; dsimp [bind, Except.bind] at run; contradiction
+      · rw [hp2] at run; dsimp [bind, Except.bind] at run
+        rcases val2 with ⟨x2, s2⟩
+        rcases hpush : pushItem (x2 >>> x1.toNat) gVerylow s2 with _ | s''
+        · rw [hpush] at run; contradiction
+        · rw [hpush] at run
+          injection run with h_eq; subst h_eq
+          exact (Devm.pop_getStor_eq hp1).trans <| (Devm.pop_getStor_eq hp2).trans <| (pushItem_getStor_eq hpush)
+⟩
+
+open Qq
+
+def Ninst.inv_expr (ξx fx : Lean.Expr) (ix : Q(Ninst)) : Lean.Elab.Tactic.TacticM Lean.Expr := do
+  let x ← Lean.Meta.synthInstance <| Lean.mkApp3 q(@Ninst.Hinv) ξx fx ix
+  pure <| Lean.mkApp4 q(@Ninst.Hinv.inv) ξx fx ix x
+
+def instInv : Lean.Elab.Tactic.TacticM Unit :=
+  Lean.Elab.Tactic.withMainContext do
+  let t ← Lean.Elab.Tactic.getMainTarget
+  have t' : Q(Prop) := t
+  match t' with
+  | ~q(@Ninst.Inv $ξx $fx $ix) =>
+    let x ← Ninst.inv_expr ξx fx ix
+    Lean.Elab.Tactic.closeMainGoal `tacName x
+  | _ => dbg_trace "Not a Ninst.Inv goal"
+
+def line_nil_inv : Lean.Elab.Tactic.TacticM Unit :=
+  Lean.Expr.apply <|
+    Lean.Expr.const (Lean.Name.str (Lean.Name.str Lean.Name.anonymous "Line") "nil_inv") []
+
+def line_cons_inv : Lean.Elab.Tactic.TacticM Unit :=
+  Lean.Expr.apply <|
+    Lean.Expr.const (Lean.Name.str (Lean.Name.str Lean.Name.anonymous "Line") "cons_inv") []
+
+partial def line_inv : Lean.Elab.Tactic.TacticM Unit :=
+  Lean.Elab.Tactic.withMainContext do
+  let t : Q(Prop) ← Lean.Elab.Tactic.getMainTarget
+  match t with
+  | ~q(@Line.Inv $ξx $fx $lx) =>
+    let lx' : Q(Line) ← Lean.Meta.whnf lx
+    match lx' with
+    | ~q([]) => line_nil_inv
+    | _ => line_cons_inv; instInv; line_inv
+  | _ => dbg_trace "Not a Line.Inv goal"
+
+elab "line_inv" : tactic => line_inv
+
 lemma weth_inv' {sevm : Sevm} {s r}
     (cond : Cond sevm.currentTarget sevm s)
     (ih : Exec.InvDepth sevm.depth sevm.currentTarget weth (Cond sevm.currentTarget)) :
@@ -891,16 +1112,15 @@ lemma weth_inv' {sevm : Sevm} {s r}
   rename Devm => s₀
   cases eq
   have cond₀ : Cond sevm.currentTarget sevm s₀ :=
-    sorry
+    Precond.state_eq cond burn.state.symm
   clear cond burn s
   revert run
-
   -- this point corresponds to the starting point of weth_inv' in Solvent.lean
   pexec fsig
   have cond₁  : Cond sevm.currentTarget sevm s₁ := by
     refine' ⟨_, _⟩
     · rw [← Line.of_inv Devm.getBal sorry h₁]; exact cond₀.nof
-    · apply Line.inv_solvent _ _ cond₀.solvent h₁ <;> sorry -- line_inv
+    · apply Line.inv_solvent _ _ cond₀.solvent h₁ <;> line_inv
   clear cond₀
   sorry
 
